Prove monad identity laws
Turns out they weren't axiomatic, we already assumed enough about the
ret and bind semantics.

Refinement/IO.v
@@ -1,5 +1,7 @@
 (* model of an IO monad *)
 
+Require Automation.
+
 Global Set Implicit Arguments.
 
 Axiom IO : Type -> Type.
@@ -19,9 +21,56 @@ Axiom ret_step : forall T (v:T) w v' w',
     io_step (Ret v) w v' w' <->
     v' = v /\ w' = w.
 
+Lemma ret_does_step : forall T (v:T) w,
+    io_step (Ret v) w v w.
+Proof.
+  intros.
+  apply ret_step; eauto.
+Qed.
+
 Axiom bind_step : forall T T' (p: IO T) (p': T -> IO T') w v' w'',
     io_step (Bind p p') w v' w'' <->
     (exists v w', io_step p w v w' /\
              io_step (p' v) w' v' w'').
 
-(* TODO: assume monad laws *)
+Lemma bind_does_step : forall T T' (p: IO T) (p': T -> IO T') w v w' v' w'',
+    io_step p w v w' ->
+    io_step (p' v) w' v' w'' ->
+    io_step (Bind p p') w v' w''.
+Proof.
+  intros.
+  eapply bind_step; eauto.
+Qed.
+
+Definition io_equiv T (step1 step2: world -> T -> world -> Prop) :=
+  forall w v w', step1 w v w' <-> step2 w v w'.
+
+Module Monad.
+
+  Import Automation.
+
+  Hint Resolve ret_does_step bind_does_step.
+
+  Theorem monad_left_id : forall T (v:T) T' (p: T -> IO T'),
+      io_equiv (io_step (Bind (Ret v) p))
+               (io_step (p v)).
+  Proof.
+    intros.
+    split; intros.
+    - apply bind_step in H; repeat deex.
+      apply ret_step in H; intuition; subst; eauto.
+    - eauto.
+  Qed.
+
+  Theorem monad_right_id : forall T (p: IO T),
+      io_equiv (io_step (Bind p Ret))
+               (io_step p).
+  Proof.
+    intros.
+    split; intros.
+    - apply bind_step in H; repeat deex.
+      apply ret_step in H0; intuition; subst; eauto.
+    - eauto.
+  Qed.
+
+End Monad.
